src/extensions/paths-new/Narrowing.v
@@ -7,68 +7,8 @@
 Set Implicit Arguments.
 
 Require Import LibLN.
-Require Import Definitions.
-Require Import Weakening.
-
-
-(** [G1] is a subenvironment of [G2], denoted [G1 subG G2],
-     if for each [x] s.t. [G2(x)=T2],
-    [G1(x) = T1] and [G1 |- T1 <: T2]. *)
-Definition subenv(G1 G2: ctx) :=
-  forall x T2, binds x T2 G2 ->
-    binds x T2 G1 \/
-    exists T1,
-      binds x T1 G1 /\ G1 ⊢ T1 <: T2.
-
-(** [G' subG G]              #<br>#
-    [ok(G', x: T)]               #<br>#
-    [―――――――――――――――――――――――――――――]  #<br>#
-    [G', x: T subG G, x: T]  #<br>#
-    Note: [ok(G)] means that [G]'s domain consists of distinct variables.
-    [ok] is defined in [TLC.LibEnv.v]. *)
-Lemma subenv_push: forall G G' x T,
-  subenv G' G ->
-  ok (G' & x ~ T) ->
-  subenv (G' & x ~ T) (G & x ~ T).
-Proof.
-  intros.
-  unfold subenv. intros xb Tb Bi. apply binds_push_inv in Bi.
-  destruct Bi as [Bi | Bi].
-  + destruct Bi as [Bi1 Bi2]. subst.
-    left. eauto.
-  + destruct Bi as [Bi1 Bi2].
-    unfold subenv in H. specialize (H xb Tb Bi2). destruct H as [Bi' | Bi'].
-    * left. eauto.
-    * right. destruct Bi' as [T' [Bi1' Bi2']].
-      exists T'. split. eauto. apply weaken_subtyp. assumption. eauto.
-Qed.
-
-(** [G ⊢ S <: U]                      #<br>#
-    [ok(G, x: S)] (see [subenv_push]) #<br>#
-    [――――――――――――――――――――――――――――――――――]  #<br>#
-    [G', x: T subG G, x: T] *)
-Lemma subenv_last: forall G x S U,
-  G ⊢ S <: U ->
-  ok (G & x ~ S) ->
-  subenv (G & x ~ S) (G & x ~ U).
-Proof.
-  intros. unfold subenv. intros y T Bi.
-  apply binds_push_inv in Bi. destruct Bi as [Bi | Bi].
-  - destruct Bi. subst. right. exists S. split; eauto using weaken_subtyp.
-  - destruct Bi. left. eauto.
-Qed.
-
-Lemma subenv_concat: forall G G' G'',
-    subenv G' G ->
-    ok (G & G'') ->
-    ok (G' & G'') ->
-    subenv (G' & G'') (G & G'').
-Proof.
-  intros. unfold subenv in *. intros y T Bi. apply binds_concat_inv in Bi.
-  destruct~ Bi. destruct H2. specialize (H y T H3). destruct~ H.
-  destruct H as [T' [Bi Hs]]. right. exists T'. split~.
-  apply~ weaken_subtyp.
-Qed.
+Require Import Coq.Program.Equality.
+Require Import Definitions Subenvironments Weakening.
 
 (** * Narrowing Lemma *)
 (** The narrowing lemma states that typing is preserved under subenvironments.
@@ -110,36 +50,39 @@ Note: for simplicity, the definition typing judgements and [ok] conditions
       are omitted from the paper formulation. *)
 Lemma narrow_rules:
   (forall G t T, G ⊢ t : T -> forall G',
-    ok G' ->
-    subenv G' G ->
+    G' ⪯ G ->
     G' ⊢ t : T)
-/\ (forall x bs P G d D, x; bs; P; G ⊢ d : D -> forall G',
-    ok G' ->
-    subenv G' G ->
-    x; bs; P; G' ⊢ d : D)
-/\ (forall x bs P G ds T, x; bs; P; G ⊢ ds :: T -> forall G',
-    ok G' ->
-    subenv G' G ->
-    x; bs; P; G' ⊢ ds :: T)
+/\ (forall z bs P G d D, z; bs; P; G ⊢ d : D -> forall G',
+    G' ⪯ G ->
+    z; bs; P; G' ⊢ d : D)
+/\ (forall z bs P G ds T, z; bs; P; G ⊢ ds :: T -> forall G',
+    G' ⪯ G ->
+    z; bs; P; G' ⊢ ds :: T)
 /\ (forall G S U, G ⊢ S <: U -> forall G',
-    ok G' ->
-    subenv G' G ->
+    G' ⪯ G ->
     G' ⊢ S <: U).
 Proof.
   apply rules_mutind; intros; eauto 4;
-    try solve [fresh_constructor; auto using subenv_push].
+    try solve [
+          match goal with
+          | [ H : _ ⪯ _ |- _ ] => destruct (subenv_implies_ok H)
+          end;
+          fresh_constructor].
+
   Case "ty_var".
+  induction H; auto;
   match goal with
-  | [ Hs: subenv _ _, Hb: binds ?x ?T _ |- _ ] =>
-    specialize (Hs x T Hb);
-    destruct_all; eauto
-  end.
+  | [ H : binds _ _ (_ & _) |- _ ] =>
+    apply binds_push_inv in H; destruct_all; subst
+  end;
+  [ eapply ty_sub; [eauto 2 | apply weaken_subtyp; trivial]
+  | apply weaken_ty_trm; auto].
 Qed.
 
 (** The narrowing lemma, formulated only for term typing. *)
 Lemma narrow_typing: forall G G' t T,
   G ⊢ t : T ->
-  subenv G' G -> ok G' ->
+  G' ⪯ G ->
   G' ⊢ t : T.
 Proof.
   intros. apply* narrow_rules.
@@ -148,7 +91,7 @@ Qed.
 (** The narrowing lemma, formulated only for subtyping. *)
 Lemma narrow_subtyping: forall G G' S U,
   G ⊢ S <: U ->
-  subenv G' G -> ok G' ->
+  G' ⪯ G ->
   G' ⊢ S <: U.
 Proof.
   intros. apply* narrow_rules.
