src/extensions/paths-new/InvertibleTyping.v
@@ -11,44 +11,159 @@ Set Implicit Arguments.
 
 Require Import LibLN.
 Require Import Coq.Program.Equality.
-Require Import Definitions.
-Require Import Narrowing.
-Require Import Binding.
-Require Import PreciseTypes.
+Require Import Definitions Narrowing PreciseTyping RecordAndInertTypes TightTyping Subenvironments.
 
-(** * Conversion into General Typing *)
+(** ** Invertible typing *)
 
-(** Precise typing implies general typing. *)
-Lemma precise_to_general: forall G t T,
-    G ⊢! t : T ->
-    G ⊢ t : T.
-Proof.
-  intros. induction H; intros; subst; eauto.
-Qed.
+(** The invertible-typing relation describes the possible types that a variable or value
+can be typed with in an inert context. For example, if [G] is inert, [G ⊢! x: {a: T}],
+and [G ⊢ T <: T'], then [G ⊢## x: {a: T'}].
 
-Lemma inv_to_tight: forall G p T,
-    G ⊢## p: T ->
-    G ⊢# trm_path p: T.
-Proof.
-  introv Ht. induction Ht; eauto. dependent induction H; eauto. constructor; auto.
-Qed.
+The purpose of invertible typing is to be easily invertible into a precise typing relation.
+To achieve that, invertible typing avoids typing cycles that could result from, for example,
+repeated applications of recursion introduction and elimination.
+For this case, invertible typing defines only recursion introduction (whereas precise typing
+defines only recursion elimination). *)
 
-(** Tight typing implies general typing. *)
-Lemma tight_to_general:
-  (forall G t T,
-     G ⊢# t : T ->
-     G ⊢ t : T) /\
-  (forall G S U,
-     G ⊢# S <: U ->
-     G ⊢ S <: U).
-Proof.
-  apply ts_mutind_ts; intros; subst; eauto using precise_to_general.
-Qed.
+(** ** Invertible typing of paths [G ⊢## p: T] *)
+
+Reserved Notation "G '⊢##' p ':' T" (at level 40, p at level 59).
+
+Inductive ty_var_inv : ctx -> path -> typ -> Prop :=
+
+(** [G ⊢! p: T]  #<br>#
+    [―――――――――――] #<br>#
+    [G ⊢## p: T]     *)
+| ty_precise_inv : forall G p T,
+  G ⊢! trm_path p : T ->
+  G ⊢## p : T
+
+(** [G ⊢## p: {a: T}] #<br>#
+    [G ⊢# T <: U]     #<br>#
+    [――――――――――――――――] #<br>#
+    [G ⊢## p: {a: U}]     *)
+| ty_dec_trm_inv : forall G p a T U,
+  G ⊢## p : typ_rcd (dec_trm a T) ->
+  G ⊢# T <: U ->
+  G ⊢## p : typ_rcd (dec_trm a U)
+
+(** [G ⊢## p: {A: T1..S1}]   #<br>#
+    [G ⊢# T2 <: T1]         #<br>#
+    [G ⊢# S1 <: S2]         #<br>#
+    [―――――――――――――――――――――] #<br>#
+    [G ⊢## p: {A: T2..S2}]     *)
+| ty_dec_typ_inv : forall G p A T1 T2 S1 S2,
+  G ⊢## p : typ_rcd (dec_typ A T1 S1) ->
+  G ⊢# T2 <: T1 ->
+  G ⊢# S1 <: S2 ->
+  G ⊢## p : typ_rcd (dec_typ A T2 S2)
+
+(** [G ⊢## p: T^p]   #<br>#
+    [―――――――――――――――] #<br>#
+    [G ⊢## p: mu(T)] *)
+| ty_bnd_inv : forall G p T,
+  G ⊢## p : open_typ_p p T ->
+  G ⊢## p : typ_bnd T
+
+(** [G ⊢## p: forall(S1)T1]          #<br>#
+    [G ⊢# S2 <: S1]            #<br>#
+    [G, y: S2 ⊢ T1^y <: T2^y]   #<br>#
+    [y fresh]                  #<br>#
+    [――――――――――――――――――――――]   #<br>#
+    [G ⊢## p: forall(S')T']            *)
+| ty_all_inv : forall G T1 T2 S1 S2 L p,
+  G ⊢## p : typ_all S1 T1 ->
+  G ⊢# S2 <: S1 ->
+  (forall y, y \notin L ->
+   G & y ~ S2 ⊢ open_typ y T1 <: open_typ y T2) ->
+  G ⊢## p : typ_all S2 T2
+
+(** [G ⊢## p : T]     #<br>#
+    [G ⊢## p : U]     #<br>#
+    [――――――――――――――――] #<br>#
+    [G ⊢## p : T /\ U]      *)
+| ty_and_inv : forall G p S1 S2,
+  G ⊢## p : S1 ->
+  G ⊢## p : S2 ->
+  G ⊢## p : typ_and S1 S2
+
+(** [G ⊢## p: S]        #<br>#
+    [G ⊢! q: {A: S..S}] #<br>#
+    [――――――――――――――――――] #<br>#
+    [G ⊢## p: q.A           *)
+| ty_path_inv : forall G p q A S,
+  G ⊢## p : S ->
+  G ⊢! trm_path q : typ_rcd (dec_typ A S S) ->
+  G ⊢## p : typ_path q A
+
+(** [G ⊢## p: T]   #<br>#
+    [―――――――――――――] #<br>#
+    [G ⊢## p: top]     *)
+| ty_top_inv : forall G p T,
+  G ⊢## p : T ->
+  G ⊢## p : typ_top
+where "G '⊢##' p ':' T" := (ty_var_inv G p T).
+
+(** ** Invertible typing for values [G ⊢##v v: T] *)
+
+Reserved Notation "G '⊢##v' v ':' T" (at level 40, v at level 59).
+
+Inductive ty_val_inv : ctx -> val -> typ -> Prop :=
+
+(** [G ⊢! v: T]    #<br>#
+    [―――――――――――――] #<br>#
+    [G ⊢##v v: T] *)
+| ty_precise_inv_v : forall G v T,
+  G ⊢! trm_val v : T ->
+  G ⊢##v v : T
+
+(** [G ⊢##v v: forall(S1)T1]          #<br>#
+    [G ⊢# S2 <: S1]             #<br>#
+    [G, y: S2 ⊢ T1^y <: T2^y]    #<br>#
+    [y fresh]                   #<br>#
+    [――――――――――――――――――――――]    #<br>#
+    [G ⊢##v v: forall(S')T']            *)
+| ty_all_inv_v : forall G v S1 S2 T1 T2 L,
+  G ⊢##v v : typ_all S1 T1 ->
+  G ⊢# S2 <: S1 ->
+  (forall y, y \notin L ->
+   G & y ~ S2 ⊢ open_typ y T1 <: open_typ y T2) ->
+  G ⊢##v v : typ_all S2 T2
+
+(** [G ⊢##v v: S]       #<br>#
+    [G ⊢! q: {A: S..S}] #<br>#
+    [――――――――――――――――――] #<br>#
+    [G ⊢##v v: q.A]         *)
+| ty_path_inv_v : forall G v S q A,
+  G ⊢##v v : S ->
+  G ⊢! trm_path q : typ_rcd (dec_typ A S S) ->
+  G ⊢##v v : typ_path q A
+
+(** [G ⊢##v v : T]        #<br>#
+    [G ⊢##v v : U]        #<br>#
+    [―――――――――――――]        #<br>#
+    [G ⊢##v v : T /\ U]        *)
+| ty_and_inv_v : forall G v T U,
+  G ⊢##v v : T ->
+  G ⊢##v v : U ->
+  G ⊢##v v : typ_and T U
+
+(** [G ⊢##v v: T]   #<br>#
+    [――――――――――――――] #<br>#
+    [G ⊢##v v: top]     *)
+| ty_top_inv_v : forall G v T,
+  G ⊢##v v : T ->
+  G ⊢##v v : typ_top
+where "G '⊢##v' v ':' T" := (ty_val_inv G v T).
+
+Hint Constructors ty_var_inv ty_val_inv.
+
+(** *** Invertible to Precise Typing [|-## to |-!] *)
 
 (** Invertible-to-precise typing for field declarations: #<br>#
-    [G |-## x: {a: T}]            #<br>#
+    [G |-## p: {a: T}]            #<br>#
     [――――――――――――――――――――――]      #<br>#
-    [exists T', G |-! x: {a: T'}]      #<br>#
+    [exists T', G |-! p: {a: T'}]      #<br>#
     [G |-# T' <: T]. *)
 Lemma invertible_to_precise_trm_dec: forall G p a T,
   G ⊢## p : typ_rcd (dec_trm a T) ->
@@ -100,7 +215,7 @@ Proof.
       eauto.
 Qed.
 
-(** * Invertible Variable Typing *)
+(** ** Invertible Subtyping Closure *)
 
 (** Invertible typing is closed under tight subtyping. *)
 Lemma invertible_typing_closure_tight: forall G p T U,
@@ -120,9 +235,15 @@ Proof.
     + pose proof (inert_unique_tight_bounds Hgd H H5) as Hu. subst. assumption.
 Qed.
 
-(** ** Tight-to-Invertible Lemma for Variables
+(** Invertible typing implies tight typing. *)
+Lemma inv_to_tight: forall G p T,
+    G ⊢## p: T ->
+    G ⊢# trm_path p: T.
+Proof.
+  introv Ht. induction Ht; eauto. dependent induction H; eauto. constructor; auto.
+Qed.
 
-       This lemma corresponds to Theorem 3.6 in the paper.
+(** *** Tight-to-Invertible Lemma for Paths [|-# to |-##]
 
        [inert G]            #<br>#
        [G ⊢# x: U]         #<br>#
@@ -158,7 +279,9 @@ Proof.
     eapply invertible_typing_closure_tight; auto.
 Qed.
 
-(** * Invertible Value Typing *)
+(** ** Invertible Value Typing *)
+
+(** *** Invertible Subtyping Closure *)
 
 (** Invertible value typing is closed under tight subtyping. *)
 Lemma invertible_typing_closure_tight_v: forall G v T U,
