src/simple-proof/proof/Narrowing.v
@@ -7,11 +7,8 @@
 Set Implicit Arguments.
 
 Require Import LibLN.
-Require Import Definitions.
-Require Import SubEnvironments.
-Require Import Weakening.
 Require Import Coq.Program.Equality.
-
+Require Import Definitions Subenvironments Weakening.
 
 (** * Narrowing Lemma *)
 (** The narrowing lemma states that typing is preserved under subenvironments.
@@ -100,21 +97,3 @@ Lemma narrow_subtyping: forall G G' S U,
 Proof.
   intros. apply* narrow_rules.
 Qed.
-
-(** The subenvironment relation [⪯] is transitive.*)
-Lemma subenv_trans : forall G1 G2 G3,
-    G1 ⪯ G2 ->
-    G2 ⪯ G3 ->
-    G1 ⪯ G3.
-Proof.
-  introv H. gen G3. induction H; intros; auto.
-  dependent induction H3.
-  - apply empty_push_inv in x. contradiction.
-  - rename x into He. apply eq_push_inv in He. destruct_all.
-    subst.
-    apply IHsubenv in H3.
-    constructor; auto.
-    apply narrow_subtyping with (G':=G) in H6; auto.
-    eapply subtyp_trans; eauto.
-Qed.
-Hint Resolve subenv_trans.
